README.md
@@ -9,4 +9,17 @@ Identify all group elements (numbers and names).
 - upXXXXX Name of element 3
 
 ## Accomplished Work
-Describe the work you have accomplished so far, and any work you have left to do. Describe also any extras you have implemented beyond the requirements.
+
+### Reverse
+
+### Grep-Naive
+
+In grep.dfy (on the grep-naive folder) we implemented the grep utility using a naive string matching algorithm. The algorithm is very simple and works by attempting to match the string over each text position, resulting in quadratic time complexity.
+
+The correctness of the grep utility is guaranteed in the "naiveSearch" method, which returns the position of the pattern in the text if it exists, or -1 if it does not. The matching of the string at each text position makes use of the "matchAt" predicate.
+
+While the "naiveSearch" method returns the position, this was only used in an earlier simpler implementation of the grep utility where we only returned a YES/NO output with the position of the first pattern occurrence (if it occurred of course).
+
+This grep utility implementation now prints all lines where the string matched with the text or "No matching lines" if there are no matches. For this, an auxiliary method "getLines" was developed, which simply splits the entire text file into a sequence of lines, which are then used to perform naive seach on each one.
+
+### Grep-KMP
